code/ecdsap256/Hacl.Impl.P256.Verify.fst
@@ -42,55 +42,6 @@ let are_r_and_s_valid r s =
   Hacl.Bignum.Base.unsafe_bool_of_limb is_s_valid
 
 
-val lemma_cancel_mont: a:S.qelem -> b:S.qelem ->
-  Lemma ((a * SM.qmont_R % S.order * b * SM.qmont_R_inv) % S.order = a * b % S.order)
-
-let lemma_cancel_mont a b =
-  calc (==) {
-    (a * SM.qmont_R % S.order * b * SM.qmont_R_inv) % S.order;
-    (==) { Math.Lemmas.paren_mul_right (a * SM.qmont_R % S.order) b SM.qmont_R_inv }
-    (a * SM.qmont_R % S.order * (b * SM.qmont_R_inv)) % S.order;
-    (==) { Math.Lemmas.lemma_mod_mul_distr_l (a * SM.qmont_R) (b * SM.qmont_R_inv) S.order }
-    (a * SM.qmont_R * (b * SM.qmont_R_inv)) % S.order;
-    (==) { Math.Lemmas.paren_mul_right a SM.qmont_R (b * SM.qmont_R_inv);
-           Math.Lemmas.swap_mul SM.qmont_R (b * SM.qmont_R_inv) }
-    (a * (b * SM.qmont_R_inv * SM.qmont_R)) % S.order;
-    (==) { Math.Lemmas.paren_mul_right b SM.qmont_R_inv SM.qmont_R }
-    (a * (b * (SM.qmont_R_inv * SM.qmont_R))) % S.order;
-    (==) { Math.Lemmas.paren_mul_right a b (SM.qmont_R_inv * SM.qmont_R) }
-    (a * b * (SM.qmont_R_inv * SM.qmont_R)) % S.order;
-    (==) { Math.Lemmas.lemma_mod_mul_distr_r (a * b) (SM.qmont_R_inv * SM.qmont_R) S.order }
-    (a * b * (SM.qmont_R_inv * SM.qmont_R % S.order)) % S.order;
-    (==) { assert_norm (SM.qmont_R_inv * SM.qmont_R % S.order = 1) }
-    (a * b) % S.order;
-  }
-
-
-val qmul_mont_lemma: s:S.qelem -> sinv:S.qelem -> b:S.qelem -> Lemma
-  (requires SM.fromDomain_ sinv == S.qinv (SM.fromDomain_ s))
-  (ensures  (sinv * SM.fromDomain_ b * SM.qmont_R_inv) % S.order == S.qinv s * b % S.order)
-
-let qmul_mont_lemma s sinv b =
-  let s_mont = SM.fromDomain_ s in
-  let b_mont = SM.fromDomain_ b in
-  calc (==) {
-    (sinv * b_mont * SM.qmont_R_inv) % S.order;
-    (==) { SM.lemmaFromDomainToDomain sinv }
-    (S.qinv s_mont * SM.qmont_R % S.order * b_mont * SM.qmont_R_inv) % S.order;
-    (==) { lemma_cancel_mont (S.qinv s_mont) b_mont }
-    (S.qinv s_mont * b_mont) % S.order;
-    (==) { PS.lemma_mont_qinv s }
-    ((S.qinv s * SM.qmont_R % S.order) * (b * SM.qmont_R_inv % S.order)) % S.order;
-    (==) { Math.Lemmas.lemma_mod_mul_distr_r
-      (S.qinv s * SM.qmont_R % S.order) (b * SM.qmont_R_inv) S.order }
-    ((S.qinv s * SM.qmont_R % S.order) * (b * SM.qmont_R_inv)) % S.order;
-    (==) { Math.Lemmas.paren_mul_right (S.qinv s * SM.qmont_R % S.order) b SM.qmont_R_inv }
-    ((S.qinv s * SM.qmont_R % S.order) * b * SM.qmont_R_inv) % S.order;
-    (==) { lemma_cancel_mont (S.qinv s) b }
-    S.qinv s * b % S.order;
-  }
-
-
 val qmul_mont: sinv:felem -> b:felem -> res:felem -> Stack unit
   (requires fun h ->
     live h sinv /\ live h b /\ live h res /\
@@ -136,8 +87,8 @@ let ecdsa_verification_get_u12 u1 u2 r s z =
   //assert (as_nat h2 sinv * SM.qmont_R_inv % S.order ==
     //S.qinv (as_nat h1 sinv * SM.qmont_R_inv % S.order));
 
-  qmul_mont_lemma (as_nat h0 s) (as_nat h1 sinv) (as_nat h0 z);
-  qmul_mont_lemma (as_nat h0 s) (as_nat h1 sinv) (as_nat h0 r);
+  SM.qmul_mont_lemma (as_nat h0 s) (as_nat h1 sinv) (as_nat h0 z);
+  SM.qmul_mont_lemma (as_nat h0 s) (as_nat h1 sinv) (as_nat h0 r);
   qmul_mont sinv z u1;
   qmul_mont sinv r u2;
   pop_frame ()
@@ -152,17 +103,25 @@ val ecdsa_verification_getx: x:felem -> pk:point -> u1:felem -> u2:felem -> Stac
     point_inv h pk /\ as_nat h u1 < pow2 256 /\ as_nat h u2 < pow2 256)
   (ensures fun h0 b h1 -> modifies (loc x) h0 h1 /\
     as_nat h1 x < S.prime /\
-   (let res = S.point_mul_double_g (as_nat h0 u1) (as_nat h0 u2) (as_point_nat h0 pk) in
-    let res = S.norm_jacob_point res in
+   (let res = S.norm_jacob_point
+     (S.point_mul_double_g (as_nat h0 u1) (as_nat h0 u2) (as_point_nat h0 pk)) in
     let (rx, _, _) = res in
     b == not (S.is_point_at_inf res) /\ as_nat h1 x == rx % S.order))
 
 let ecdsa_verification_getx x pk u1 u2 =
   push_frame ();
   let res = create_point () in
+  let h0 = ST.get () in
   point_mul_double_g res u1 u2 pk;
+  let h1 = ST.get () in
+  assert (from_mont_point (as_point_nat h1 res) ==
+    S.point_mul_double_g (as_nat h0 u1) (as_nat h0 u2) (as_point_nat h0 pk));
   norm_jacob_point res res;
+  let h2 = ST.get () in
+  assert (as_point_nat h2 res ==
+    S.norm_jacob_point (from_mont_point (as_point_nat h1 res)));
   let is_res_point_at_inf = is_point_at_inf_vartime res in
+  assert (is_res_point_at_inf == S.is_point_at_inf (as_point_nat h2 res));
   let res_x = getx res in
   qmod_short x res_x;
   pop_frame ();
